hoare_sound.v
@@ -16,8 +16,7 @@ Definition hoare_sound (T: FirstOrderLogic): Prop :=
 Lemma aeval_aexp'_denote: forall st La a,
   aeval a st = aexp'_denote (st, La) (ainj a).
 Proof.
-Admitted.
-(*   intros.
+  intros.
   induction a; simpl.
   + reflexivity.
   + reflexivity.
@@ -27,13 +26,12 @@ Admitted.
     reflexivity.
   + rewrite IHa1, IHa2.
     reflexivity.
-Qed. *)
+Qed.
 
 Lemma beval_bexp'_denote: forall st La b,
   beval b st <-> bexp'_denote (st, La) (binj b).
 Proof.
-Admitted.
-(*   intros.
+  intros.
   induction b; simpl.
   + tauto.
   + tauto.
@@ -45,7 +43,7 @@ Admitted.
     tauto.
   + tauto.
   + tauto.
-Qed. *)
+Qed.
 
 
 (** We will prove that if the logic for assertion derivation is sound, then the
@@ -66,25 +64,55 @@ Lemma hoare_seq_sound : forall (P Q R QB QC RB RC: Assertion) (c1 c2: com),
   |== {{Q}} c2 {{R}} {{RB}} {{RC}}->
   |== {{P}} c1;;c2 {{R}} {{RB}} {{RC}}.
 Proof.
-Admitted.
-(*   unfold valid.
+  unfold valid.
   intros.
   simpl in H2.
-  unfold Relation_Operators.concat in H2.
-  destruct H2 as [st1' [? ?]].
-  specialize (H _ _ _ H1 H2).
-  specialize (H0 _ _ _ H H3).
-  exact H0.
-Qed. *)
+  unfold seq_sem in H2.
+  destruct H2.
+  + destruct H2 as [st1' [? ?]].
+    specialize (H _ _ _ H1 H2).
+    specialize (H0 _ _ _ H H3).
+    exact H0.
+  + destruct H2.
+    unfold not in H3.
+    destruct H3.
+    reflexivity.
+Qed.
 
 Lemma hoare_skip_sound : forall P,
   |== {{P}} Skip {{P}}{{{[BFalse]}}}{{{[BFalse]}}}.
 Proof.
-Admitted.
-(*   unfold valid.
+  unfold valid.
   intros.
   simpl in H0.
-  unfold Relation_Operators.id in H0.
+  unfold skip_sem in H0.
+  destruct H0.
+  rewrite <- H0.
+  exact H.
+Qed.
+
+Lemma hoare_break_sound : forall P,
+  |== {{P}} Skip {{{[BFalse]}}}{{P}}{{{[BFalse]}}}.
+Proof.
+Admitted.
+(*unfold valid.
+  intros.
+  simpl in H0.
+  unfold skip_sem in H0.
+  destruct H0.
+  rewrite <- H0.
+  exact H.
+Qed. *)
+
+Lemma hoare_continue_sound : forall P,
+  |== {{P}} Skip {{{[BFalse]}}}{{{[BFalse]}}}{{P}}.
+Proof.
+Admitted.
+(*unfold valid.
+  intros.
+  simpl in H0.
+  unfold skip_sem in H0.
+  destruct H0.
   rewrite <- H0.
   exact H.
 Qed. *)
@@ -94,16 +122,11 @@ Lemma hoare_if_sound : forall P Q QB QC(b: bexp) c1 c2,
   |== {{ P AND NOT {[b]} }} c2 {{ Q }} {{ QB }} {{ QC }} ->
   |== {{ P }} If b Then c1 Else c2 EndIf {{ Q }} {{ QB }} {{ QC }}.
 Proof.
-Admitted.
-(* 
   unfold valid.
   intros.
   simpl in H2.
   unfold if_sem in H2.
-  unfold Relation_Operators.union,
-         Relation_Operators.intersection,
-         Relation_Operators.filter1 in H2.
-  destruct H2 as [[? ?] | [? ?]].
+  repeat destruct H2.
   + apply H with st1.
     - simpl.
       pose proof beval_bexp'_denote st1 La b.
@@ -111,16 +134,44 @@ Admitted.
     - exact H2.
   + apply H0 with st1.
     - simpl.
-      simpl in H3.
       pose proof beval_bexp'_denote st1 La b.
       tauto.
     - exact H2.
-Qed. *)
+Qed.
 
 Lemma hoare_while_sound : forall I P(b: bexp) c,
   |== {{ I AND {[b]} }} c {{I}} {{P}} {{I}} ->
   |== {{ I }} While b Do c EndWhile {{ P OR (I AND NOT {[b]}) }} {{{[BFalse]}}} {{{[BFalse]}}}.
 Proof.
+  unfold valid.
+  intros.
+  simpl in H1.
+  unfold loop_sem1 in H1.
+  destruct H1 as [n ?].
+  revert st1 H0 H1; induction n; intros.
+  + simpl in H1.
+    repeat destruct H1.
+    simpl.
+    right.
+    pose proof beval_bexp'_denote st1 La b.
+    rewrite <- H1.
+    tauto.
+  + simpl in H1.
+    repeat destruct H1.
+    - apply IHn with x.
+      * assert ((st1, La) |== I AND {[b]}).
+        {
+          simpl.
+          pose proof beval_bexp'_denote st1 La b.
+          tauto.
+        }
+        specialize (H _ _ _ H5 H1).
+        exact H.
+      * split; [exact H4|exact H2].
+    - simpl in H1.
+      
+      
+
 Admitted.
 (*   unfold valid.
   intros.
@@ -152,9 +203,29 @@ Admitted.
     - exact H2.
 Qed.
  *)
+
+Lemma hoare_for_sound : forall U I IT P c1 (b:bexp) c2 c3,
+  |== {{U}} c1 {{I}}{{{[BFalse]}}}{{{[BFalse]}}} ->
+  |== {{I AND {[b]}}} c3 {{IT}}{{P}}{{IT}} ->
+  |== {{IT}} c2 {{I}}{{{[BFalse]}}}{{{[BFalse]}}} ->
+  |== {{U}} For( c1; b; c2) c3 EndFor {{P OR I AND NOT {[b]}}}{{{[BFalse]}}}{{{[BFalse]}}}.
+Proof.
+  unfold valid.
+  intros.
+Admitted.
+
+Lemma hoare_dowhile_sound : forall U I P0 P1 (b:bexp) c,
+  |== {{U}} c {{I}}{{P0}}{{I}} ->
+  |== {{I AND {[b]}}} c {{I}}{{P1}}{{I}} ->
+  |== {{U}} Do c While b EndWhile {{P0 OR P1 OR I AND NOT {[b]}}}{{{[BFalse]}}}{{{[BFalse]}}}.
+Proof.
+  unfold valid.
+  intros.
+Admitted.
+
 Lemma Assertion_sub_spec: forall st1 st2 La (P: Assertion) (X: var) (E: aexp),
   st2 X = aexp'_denote (st1, La) E ->
-  (forall Y : var, X <> Y -> st1 Y = st2 Y) ->
+  (forall Y : var, X <> Y -> st1 Y = st2 Y) /\ EK_Normal = EK_Normal->
   ((st1, La) |== P[ X |-> E]) <-> ((st2, La) |== P).
 Proof.
   intros.
@@ -167,17 +238,24 @@ Proof.
 Lemma hoare_asgn_bwd_sound : forall P (X: var) (E: aexp),
   |== {{ P [ X |-> E] }} X ::= E {{ P }}{{{[BFalse]}}}{{{[BFalse]}}}.
 Proof.
-Admitted.
-(*   unfold valid.
+  unfold valid.
   intros.
   simpl in H0.
+  unfold asgn_sem in H0.
   destruct H0.
   pose proof aeval_aexp'_denote st1 La E.
   rewrite H2 in H0.
-  pose proof Assertion_sub_spec st1 st2 La P X E H0 H1.
-  tauto.
+  pose proof Assertion_sub_spec st1 st2 La P X E H0.
+  apply H3.
+  + split.
+    - intros.
+      specialize (H1 Y H4).
+      destruct H1.
+      exact H1.
+    - reflexivity.
+  + exact H.
 Qed.
- *)
+
 Lemma hoare_consequence_sound : forall (T: FirstOrderLogic) (P P' Q Q' QB QB' QC QC': Assertion) c,
   FOL_sound T ->
   P |-- P' ->
@@ -187,8 +265,7 @@ Lemma hoare_consequence_sound : forall (T: FirstOrderLogic) (P P' Q Q' QB QB' QC
   QC' |-- QC ->
   |== {{P}} c {{Q}} {{QB}} {{QC}}.
 Proof.
-Admitted.
-(*   intros.
+  intros.
   unfold FOL_sound in H.
   unfold derives in H0, H2.
   apply H in H0.
@@ -203,16 +280,15 @@ Admitted.
     specialize (H0 (st1, La)).
     tauto.
   }
-  pose proof H1 _ _ _ H5 H4.
+  specialize (H1 _ _ _ H7 H6).
   specialize (H2 (st2, La)).
   tauto.
-Qed. *)
+Qed.
 
 Theorem Hoare_logic_soundness: forall (T: FirstOrderLogic) (TS: FOL_sound T),
   hoare_sound T.
 Proof.
-Admitted.
-(*   intros.
+  intros.
   unfold hoare_sound.
   intros.
   remember ({{P}} c {{Q}}{{QB}}{{QC}}) as Tr.
@@ -227,9 +303,20 @@ Admitted.
     - exact IHprovable2.
   + apply hoare_while_sound.
     exact IHprovable.
+  + apply hoare_for_sound with IT.
+    - exact IHprovable1.
+    - exact IHprovable2.
+    - exact IHprovable3.
+  + apply hoare_dowhile_sound.
+    - exact IHprovable1.
+    - exact IHprovable2.
   + apply hoare_asgn_bwd_sound.
   + pose proof hoare_consequence_sound T P P' Q Q' QB0 QB' QC0 QC' c TS H IHprovable H1 H2 H3.
     exact H4.
-Qed. *)
+  + apply hoare_continue_sound.
+  + apply hoare_break_sound.
+Qed.
+
+
 
 (* Thu Apr 25 12:10:27 UTC 2019 *)
